
\section{Frozen core CI}

Let us start from the following representation of the Hamiltonian with restricted parameters:
\begin{equation}\label{eq:ham}
      \hat{\mathcal{H}}_\text{elec} = \sum_{pq}^K h_{pq} \hat{E}_{pq} + \frac{1}{2} \sum_{pqrs}^K g_{pqrs} \hat{e}_{pqrs}
  \end{equation}

We freeze the first X orbitals and fill them with electrons pairs. And define L as $L=K-X$.  Let us call the Hamiltonian in this space $\hat{\mathcal{H}}^{f}_\text{elec}$.
We define $\hat{{H}}^{L}$ as the hamiltonian in the new product Fock space of Fock space alpha with L orbitals and $N_\alpha - X$ electrons abd Fock space beta with L orbitals and $N_\beta - X$. Let us define $\hat{{H}}^{X}$ as the Hamiltonian in the working exclusively on the frozen orbitals and $\hat{{H}}^{Q}$ as missing Hamiltonian elements in complete frozen Fock space.

\begin{equation}
  \hat{\mathcal{H}}^{f}_\text{elec} = \hat{{H}}^{L} + \hat{{H}}^{X} + \hat{{H}}^{Q}
\end{equation}

For $\hat{{H}}^{L}$ we find no changes to FCI Hamiltonian in its Fock space.
\begin{equation}
  \hat{{H}}^{L} = \sum_{pq}^L k_{pq} \hat{E}_{pq} + \frac{1}{2} \sum_{pqrs}^L g_{pqrs} \hat{E}_{pq} \hat{E}_{rs}
\end{equation}

For $\hat{{H}}^{X}$ all orbitals are occupied hence we find for any $\ket{I}$:
\begin{align}
 \bra{I}  \hat{{H}}^{X} \ket{I} &= \sum^{X}_{p}  h_{pp} * (\braket{\alpha}{\alpha} + \braket{\beta}{\beta}) + \frac{1}{2} g_{pppp} * (\braket{\alpha \beta}{\beta \alpha} + \braket{\beta \alpha}{\alpha \beta})  \\
   & +  \frac{1}{2} \sum^{X}_{p<q}  (g_{ppqq} + g_{qqpp}) * (\braket{\alpha \beta}{\beta \alpha} + \braket{\beta \alpha}{\alpha \beta} + \braket{\alpha \alpha}{\alpha \alpha} + \braket{\beta \beta}{\beta \beta}) \\
    & -  \frac{1}{2} \sum^{X}_{p<q} (g_{pqqp} + g_{qppq}) * (\braket{\alpha \alpha}{\alpha \alpha} + \braket{\beta \beta}{\beta \beta}) \\
    & = \sum^{X}_{p} 2 h_{pp} + g_{pppp} + \sum^{X}_{p<q} 2g_{ppqq} + 2g_{qqpp} - g_{pqqp} - g_{qppq} \\
    \bra{I} \hat{{H}}^{X} \ket{J} &= 0
\end{align}


For $\hat{{H}}^{Q}$ we find :
\begin{align}
   \hat{{H}}^{Q}  &= \sum_{pq}^L \Big(\sum^{X}_r g_{pqrr} + g_{rrpq} - \frac{g_{prrq} + g_{rpqr}}{2}  \Big)  \hat{E}_{pq}
\end{align}

This means we can modify the one electron integral from $\hat{{H}}^{L}$ with $\hat{{H}}^{Q}$.

\begin{align}
   \hat{{H}}^{LQ}  &=  \hat{{H}}^{L} + \hat{{H}}^{Q} \\
                  &=  \sum_{pq}^L \Big(k_{pq} + \sum^{X}_r g_{pqrr} + g_{rrpq} - \frac{g_{prrq} + g_{rpqr}}{2} \Big) \hat{E}_{pq} + \frac{1}{2} \sum_{pqrs}^L g_{pqrs} \hat{E}_{pq} \hat{E}_{rs}
\end{align}
We can then perform the FCI algorithm in $\hat{{H}}^{L}$'s Fock Space, and then perform diagonal correction with the evaluations from $\hat{{H}}^{X}$.


\subsection{Unrestricted Frozen Core CI}
  \begin{align}
    \bra{I} \hat{{H}}^{X} \ket{I} &= \sum^{X}_{p} h_{pp}^\alpha +  h_{pp}^\beta + g_{pppp}^{\alpha \beta} + \sum^{X}_{p<q} g_{ppqq}^{\alpha \beta} + g_{qqpp}^{\alpha \beta} \\
    &+ \frac{g_{ppqq}^\beta + g_{qqpp}^\beta  - g_{pqqp}^\beta - g_{qppq}^\beta }{2} + \frac{g_{ppqq}^\alpha + g_{qqpp}^\alpha - g_{pqqp}^\alpha - g_{qppq}^\alpha }{2}
   \end{align}

   For $\hat{{H}}^{Q}$ we find :
   \begin{align}
      \hat{{H}}^{Q}  &= \sum_{pq}^L \Big(\sum^{X}_r g_{pqrr} + g_{rrpq} - \frac{g_{prrq} + g_{rpqr}}{2}  \Big)  \hat{a}^{\alpha \dagger}_p \hat{a}^{\alpha}_q 
   \end{align}

\subsection{RDMs}

We have restrictedly frozen the first X orbitals hence for 1-RDMs we find for the first X indices:
\begin{align}
  \forall p &\in [0,X[ \\
  & D_{pp} = \bra{\Psi} E_{pp} \ket{\Psi} = \braket{\Psi}{\Psi} + \braket{\Psi}{\Psi} \\
  & D_{pp}^\alpha = D_{pp}^\beta = 1
\end{align}

For 2-RDMs for the first X indices we find:
\begin{align}
  \forall p,q \in & [0,X[ \\
  & d^{\sigma \sigma \sigma \sigma}_{ppqq} = \braket{\Psi}{\Psi} = 1 \\
  & d^{\sigma \sigma \sigma \sigma}_{pqqp} = - 1 \\
  & d^{\sigma \sigma \sigma \sigma}_{pppp} = 0 \\
  & d^{\sigma \sigma \tau \tau}_{ppqq} = 1 \\
  & d^{\sigma \sigma \tau \tau}_{pppp} = 1 \\
  & d_{ppqq} = 4 \\
  & d_{pppp} = 2 \\
  \forall p \in & [0, X[ q,r \notin [0, X[ \\
  & d^{\sigma \sigma \sigma \sigma}_{ppqr} = \bra{\Psi} E_{qr}^{\sigma} \ket{\Psi} = D_{qr}^{\sigma} \\
  & d^{\sigma \sigma \sigma \sigma}_{pqrp} = - D_{qr}^{\sigma} \\
  & d^{\sigma \sigma \tau \tau}_{ppqr} = D_{qr}^{\tau} \\
  & d^{\tau \tau \sigma \sigma}_{ppqr} = D_{qr}^{\sigma} \\
  & d_{ppqr} = 2 D_{qr} \\
  & d_{pqrp} = - D_{qr}
\end{align}
